Added Two Lemmas for List_Concat

src/data-types/binary-tree/BinaryTree.dfy
@@ -3,8 +3,13 @@ include "../list/List.dfy"
 datatype Leaf = Nil
 datatype BinaryTree<T> = Leaf | Node(left:BinaryTree<T>, data:T, right:BinaryTree<T>)
 
-function method BinaryTree_InOrderElems(tree:BinaryTree<T>) : List<T>
+// ---------------------- Function Methods ---------------------- //
+
+function method BinaryTree_InOrderElems(tree:BinaryTree<T>) : (result:List<T>)
   decreases tree
+  requires binarytree_ordered(tree)
+  // Mismos elementos el tree que el result
+  // Result esté ordenado
 {
   match tree {
     case Leaf => List_Empty
@@ -12,8 +17,19 @@ function method BinaryTree_InOrderElems(tree:BinaryTree<T>) : List<T>
   }
 }
 
-function method BinaryTree_Insert(tree:BinaryTree<T>, x:int): BinaryTree<T>
+function method BinaryTree_Elems(tree:BinaryTree<T>): seq<T>
   decreases tree
+{
+  match tree {
+    case Leaf => []
+    case Node(l, d, r) => BinaryTree_Elems(l) + [d] + BinaryTree_Elems(r)
+  }
+}
+
+function method BinaryTree_Insert(tree:BinaryTree<T>, x:T): (result:BinaryTree<T>)
+  decreases tree
+  requires binarytree_ordered(tree)
+  ensures binarytree_ordered(result)
 {
   match tree {
     case Leaf => Node(Leaf, x, Leaf)
@@ -32,3 +48,38 @@ function method BinaryTree_Mirror(tree:BinaryTree<T>): BinaryTree<T>
     case Node(l, d, r) => Node(BinaryTree_Mirror(r), d, BinaryTree_Mirror(l))
   }
 }
+
+// ---------------------- Predicates ---------------------- //
+
+predicate binarytree_ordered(tree:BinaryTree<T>) 
+  decreases tree
+{
+  match tree {
+    case Leaf => true
+    case Node(l, d, r) => 
+      binarytree_value_is_greater_than_root(l, d) &&
+      binarytree_value_is_lesser_than_root(r, d) &&
+      binarytree_ordered(l) &&
+      binarytree_ordered(r)
+  }
+}
+
+predicate binarytree_value_is_greater_than_root(tree:BinaryTree<T>, value:T)
+  decreases tree
+{
+  match tree {
+    case Leaf => true
+    case Node(l, root, r) => value > root
+  }
+}
+
+predicate binarytree_value_is_lesser_than_root(tree:BinaryTree<T>, value:T)
+  decreases tree
+{
+  match tree {
+    case Leaf => true
+    case Node(l, root, r) => value < root
+  }
+}
+
+// ------------------------ Lemmas ------------------------ //
