src/data-types/list/List.dfy
@@ -3,12 +3,16 @@ type T = int
 datatype List_Empty = Nil
 datatype List<T> = List_Empty | Cons(head:T, tail:List<T>)
 
+// ------------------------- Functions -------------------------- //
+
 function create(): List<T>
 {
   List_Empty
 }
 
-function method List_Size(list:List<T>) : int
+// ---------------------- Function Methods ---------------------- //
+
+function method {:tailrecursion true} List_Size(list:List<T>) : int
   decreases list
 {
   match list {
@@ -28,10 +32,16 @@ function method List_Insert(list:List<T>, x:T) : List<T>
 
 function method List_Concat(a:List<T>, b:List<T>) : List<T>
   decreases a
+  ensures List_Elems(List_Concat(a, b)) == List_Elems(a) + List_Elems(b)
+  ensures List_Size(List_Concat(a, b)) == List_Size(a) + List_Size(b)
 {
   match a {
     case List_Empty => b
-    case Cons(h, t) => Cons(h, List_Concat(t, b))
+    case Cons(h, t) =>
+      match b {
+        case List_Empty => a
+        case Cons(hb, tb) => Cons(h, List_Concat(t, Cons(hb, tb)))
+    }
   }
 }
 
@@ -49,7 +59,9 @@ function method List_Tail(xs:List<T>): List<T>
     case Cons(y, ys) => ys
 }
 
-method List_Print(a:List<T>) 
+// ------------------------- Methods -------------------------- //
+
+method {:tailrecursion true} List_Print(a:List<T>) 
   decreases a
 {
   match a {
@@ -64,5 +76,76 @@ method List_Print(a:List<T>)
       print h, ", ";
       List_Print(t);
     }
+  }
+}
+
+function method List_Elems(a:List<T>): seq<T>
+  decreases a
+{
+  match a {
+    case List_Empty => []
+    case Cons(h, t) => [h] + List_Elems(t)
+  }
+}
+
+// ---------------------- Predicates ---------------------- //
+
+predicate list_ascending_order(list:List<T>) 
+  decreases list
+{
+  match list {
+    case List_Empty => true
+    case Cons(h, List_Empty) => true
+    case Cons(h, Cons(ht, t)) => h <= ht && list_ascending_order(t)
+  }
+}
+
+// ------------------------ Lemmas ------------------------ //
+
+lemma {:induction false} ConcatElemsLemma(a:List<T>, b:List<T>)
+  ensures List_Elems(List_Concat(a, b)) == List_Elems(a) + List_Elems(b)
+  decreases a, b
+{
+  match a {
+    case List_Empty =>
+      calc == {
+        List_Elems(List_Concat(a, b));
+          { assert List_Elems(a) + List_Elems(b) == List_Elems(b); }
+        [] + List_Elems(b);
+          { assert List_Elems(a) == []; }
+        List_Elems(a) + List_Elems(b);
+      }
+    case Cons(ha, ta) =>
+      calc == {
+        List_Elems(List_Concat(a, b));
+          { assert List_Elems(List_Concat(a, b)) == List_Elems(Cons(ha, List_Empty)) + List_Elems(List_Concat(ta, b)); }
+        List_Elems(Cons(ha, List_Empty)) + List_Elems(List_Concat(ta, b));
+          { ConcatElemsLemma(ta, b); }
+        List_Elems(a) + List_Elems(b);
+      }
+  }
+}
+
+lemma {:induction false} ConcatSizeLemma(a:List<T>, b:List<T>)
+  ensures List_Size(List_Concat(a, b)) == List_Size(a) + List_Size(b)
+  decreases a, b
+{
+  match a {
+    case List_Empty =>
+      calc == {
+        List_Size(List_Concat(a, b));
+          { assert List_Size(a) + List_Size(b) == List_Size(b); }
+        0 + List_Size(b);
+          { assert List_Size(a) == 0; }
+        List_Size(a) + List_Size(b);
+      }
+    case Cons(ha, ta) =>
+      calc == {
+        List_Size(List_Concat(a, b));
+          { assert List_Size(List_Concat(a, b)) == List_Size(Cons(ha, List_Empty)) + List_Size(List_Concat(ta, b)); }
+        List_Size(Cons(ha, List_Empty)) + List_Size(List_Concat(ta, b));
+          { ConcatSizeLemma(ta, b); }
+        List_Size(a) + List_Size(b);
+      }
   }
 }
